converted to Isar script, simplifying some results

src/HOL/Wellfounded_Recursion.thy
@@ -1,19 +1,20 @@
-(*  Title:      HOL/Wellfounded_Recursion.thy
-    ID:         $Id$
+(*  ID:         $Id$
     Author:     Tobias Nipkow
     Copyright   1992  University of Cambridge
-
-Well-founded Recursion
 *)
 
-Wellfounded_Recursion = Transitive_Closure + 
+header {*Well-founded Recursion*}
+
+theory Wellfounded_Recursion
+imports Transitive_Closure
+begin
 
 consts
   wfrec_rel :: "('a * 'a) set => (('a => 'b) => 'a => 'b) => ('a * 'b) set"
 
 inductive "wfrec_rel R F"
-intrs
-  wfrecI "ALL z. (z, x) : R --> (z, g z) : wfrec_rel R F ==>
+intros
+  wfrecI: "ALL z. (z, x) : R --> (z, g z) : wfrec_rel R F ==>
             (x, F g x) : wfrec_rel R F"
 
 constdefs
@@ -33,8 +34,329 @@ constdefs
   wfrec :: "('a * 'a) set => (('a => 'b) => 'a => 'b) => 'a => 'b"
   "wfrec R F == %x. THE y. (x, y) : wfrec_rel R (%f x. F (cut f R x) x)"
 
-axclass
-  wellorder < linorder
-  wf "wf {(x,y::'a::ord). x<y}"
+axclass wellorder \<subseteq> linorder
+  wf: "wf {(x,y::'a::ord). x<y}"
+
+
+lemma wfUNIVI: 
+   "(!!P x. (ALL x. (ALL y. (y,x) : r --> P(y)) --> P(x)) ==> P(x)) ==> wf(r)"
+by (unfold wf_def, blast)
+
+text{*Restriction to domain @{term A}.  
+  If @{term r} is well-founded over @{term A} then @{term "wf r"}*}
+lemma wfI: 
+ "[| r <= A <*> A;   
+     !!x P. [| ALL x. (ALL y. (y,x) : r --> P y) --> P x;  x:A |] ==> P x |]   
+  ==>  wf r"
+by (unfold wf_def, blast)
+
+lemma wf_induct: 
+    "[| wf(r);           
+        !!x.[| ALL y. (y,x): r --> P(y) |] ==> P(x)  
+     |]  ==>  P(a)"
+by (unfold wf_def, blast)
+
+lemma wf_not_sym [rule_format]: "wf(r) ==> ALL x. (a,x):r --> (x,a)~:r"
+by (erule_tac a=a in wf_induct, blast)
+
+(* [| wf r;  ~Z ==> (a,x) : r;  (x,a) ~: r ==> Z |] ==> Z *)
+lemmas wf_asym = wf_not_sym [elim_format]
+
+lemma wf_not_refl [simp]: "wf(r) ==> (a,a) ~: r"
+by (blast elim: wf_asym)
+
+(* [| wf r;  (a,a) ~: r ==> PROP W |] ==> PROP W *)
+lemmas wf_irrefl = wf_not_refl [elim_format]
+
+text{*transitive closure of a well-founded relation is well-founded! *}
+lemma wf_trancl: "wf(r) ==> wf(r^+)"
+apply (subst wf_def, clarify)
+apply (rule allE, assumption)
+  --{*Retains the universal formula for later use!*}
+apply (erule mp)
+apply (erule_tac a = x in wf_induct)
+apply (blast elim: tranclE)
+done
+
+lemma wf_converse_trancl: "wf (r^-1) ==> wf ((r^+)^-1)"
+apply (subst trancl_converse [symmetric])
+apply (erule wf_trancl)
+done
+
+
+subsubsection{*Minimal-element characterization of well-foundedness*}
+
+lemma lemma1: "wf r ==> x:Q --> (EX z:Q. ALL y. (y,z):r --> y~:Q)"
+apply (unfold wf_def)
+apply (drule spec)
+apply (erule mp [THEN spec], blast)
+done
+
+lemma lemma2: "(ALL Q x. x:Q --> (EX z:Q. ALL y. (y,z):r --> y~:Q)) ==> wf r"
+apply (unfold wf_def, clarify)
+apply (drule_tac x = "{x. ~ P x}" in spec, blast)
+done
+
+lemma wf_eq_minimal: "wf r = (ALL Q x. x:Q --> (EX z:Q. ALL y. (y,z):r --> y~:Q))"
+by (blast intro!: lemma1 lemma2)
+
+subsubsection{*Other simple well-foundedness results*}
+
+
+text{*Well-foundedness of subsets*}
+lemma wf_subset: "[| wf(r);  p<=r |] ==> wf(p)"
+apply (simp (no_asm_use) add: wf_eq_minimal)
+apply fast
+done
+
+text{*Well-foundedness of the empty relation*}
+lemma wf_empty [iff]: "wf({})"
+by (simp add: wf_def)
+
+text{*Well-foundedness of insert*}
+lemma wf_insert [iff]: "wf(insert (y,x) r) = (wf(r) & (x,y) ~: r^*)"
+apply (rule iffI)
+ apply (blast elim: wf_trancl [THEN wf_irrefl]
+              intro: rtrancl_into_trancl1 wf_subset 
+                     rtrancl_mono [THEN [2] rev_subsetD])
+apply (simp add: wf_eq_minimal, safe)
+apply (rule allE, assumption, erule impE, blast) 
+apply (erule bexE)
+apply (rename_tac "a", case_tac "a = x")
+ prefer 2
+apply blast 
+apply (case_tac "y:Q")
+ prefer 2 apply blast
+apply (rule_tac x = "{z. z:Q & (z,y) : r^*}" in allE)
+ apply assumption
+apply (erule_tac V = "ALL Q. (EX x. x : Q) --> ?P Q" in thin_rl) 
+  --{*essential for speed*}
+txt{*Blast_tac with new substOccur fails*}
+apply (fast intro: converse_rtrancl_into_rtrancl)
+done
+
+text{*Well-foundedness of image*}
+lemma wf_prod_fun_image: "[| wf r; inj f |] ==> wf(prod_fun f f ` r)"
+apply (simp only: wf_eq_minimal, clarify)
+apply (case_tac "EX p. f p : Q")
+apply (erule_tac x = "{p. f p : Q}" in allE)
+apply (fast dest: inj_onD, blast)
+done
+
+
+subsubsection{*Well-Foundedness Results for Unions*}
+
+text{*Well-foundedness of indexed union with disjoint domains and ranges*}
+
+lemma wf_UN: "[| ALL i:I. wf(r i);  
+         ALL i:I. ALL j:I. r i ~= r j --> Domain(r i) Int Range(r j) = {}  
+      |] ==> wf(UN i:I. r i)"
+apply (simp only: wf_eq_minimal, clarify)
+apply (rename_tac A a, case_tac "EX i:I. EX a:A. EX b:A. (b,a) : r i")
+ prefer 2
+ apply force 
+apply clarify
+apply (drule bspec, assumption)  
+apply (erule_tac x="{a. a:A & (EX b:A. (b,a) : r i) }" in allE)
+apply (blast elim!: allE)  
+done
+
+lemma wf_Union: 
+ "[| ALL r:R. wf r;  
+     ALL r:R. ALL s:R. r ~= s --> Domain r Int Range s = {}  
+  |] ==> wf(Union R)"
+apply (simp add: Union_def)
+apply (blast intro: wf_UN)
+done
+
+(*Intuition: we find an (R u S)-min element of a nonempty subset A
+             by case distinction.
+  1. There is a step a -R-> b with a,b : A.
+     Pick an R-min element z of the (nonempty) set {a:A | EX b:A. a -R-> b}.
+     By definition, there is z':A s.t. z -R-> z'. Because z is R-min in the
+     subset, z' must be R-min in A. Because z' has an R-predecessor, it cannot
+     have an S-successor and is thus S-min in A as well.
+  2. There is no such step.
+     Pick an S-min element of A. In this case it must be an R-min
+     element of A as well.
+
+*)
+lemma wf_Un:
+     "[| wf r; wf s; Domain r Int Range s = {} |] ==> wf(r Un s)"
+apply (simp only: wf_eq_minimal, clarify) 
+apply (rename_tac A a)
+apply (case_tac "EX a:A. EX b:A. (b,a) : r") 
+ prefer 2
+ apply simp
+ apply (drule_tac x=A in spec)+
+ apply blast 
+apply (erule_tac x="{a. a:A & (EX b:A. (b,a) : r) }" in allE)+
+apply (blast elim!: allE)  
+done
+
+subsubsection {*acyclic*}
+
+lemma acyclicI: "ALL x. (x, x) ~: r^+ ==> acyclic r"
+by (simp add: acyclic_def)
+
+lemma wf_acyclic: "wf r ==> acyclic r"
+apply (simp add: acyclic_def)
+apply (blast elim: wf_trancl [THEN wf_irrefl])
+done
+
+lemma acyclic_insert [iff]:
+     "acyclic(insert (y,x) r) = (acyclic r & (x,y) ~: r^*)"
+apply (simp add: acyclic_def trancl_insert)
+apply (blast intro: rtrancl_trans)
+done
+
+lemma acyclic_converse [iff]: "acyclic(r^-1) = acyclic r"
+by (simp add: acyclic_def trancl_converse)
+
+lemma acyclic_impl_antisym_rtrancl: "acyclic r ==> antisym(r^*)"
+apply (simp add: acyclic_def antisym_def)
+apply (blast elim: rtranclE intro: rtrancl_into_trancl1 rtrancl_trancl_trancl)
+done
+
+(* Other direction:
+acyclic = no loops
+antisym = only self loops
+Goalw [acyclic_def,antisym_def] "antisym( r^* ) ==> acyclic(r - Id)
+==> antisym( r^* ) = acyclic(r - Id)";
+*)
+
+lemma acyclic_subset: "[| acyclic s; r <= s |] ==> acyclic r"
+apply (simp add: acyclic_def)
+apply (blast intro: trancl_mono)
+done
+
+
+subsection{*Well-Founded Recursion*}
+
+text{*cut*}
+
+lemma cuts_eq: "(cut f r x = cut g r x) = (ALL y. (y,x):r --> f(y)=g(y))"
+by (simp add: expand_fun_eq cut_def)
+
+lemma cut_apply: "(x,a):r ==> (cut f r a)(x) = f(x)"
+by (simp add: cut_def)
+
+text{*Inductive characterization of wfrec combinator; for details see:  
+John Harrison, "Inductive definitions: automation and application"*}
+
+lemma wfrec_unique: "[| adm_wf R F; wf R |] ==> EX! y. (x, y) : wfrec_rel R F"
+apply (simp add: adm_wf_def)
+apply (erule_tac a=x in wf_induct) 
+apply (rule ex1I)
+apply (rule_tac g = "%x. THE y. (x, y) : wfrec_rel R F" in wfrec_rel.wfrecI)
+apply (fast dest!: theI')
+apply (erule wfrec_rel.cases, simp)
+apply (erule allE, erule allE, erule allE, erule mp)
+apply (fast intro: the_equality [symmetric])
+done
+
+lemma adm_lemma: "adm_wf R (%f x. F (cut f R x) x)"
+apply (simp add: adm_wf_def)
+apply (intro strip)
+apply (rule cuts_eq [THEN iffD2, THEN subst], assumption)
+apply (rule refl)
+done
+
+lemma wfrec: "wf(r) ==> wfrec r H a = H (cut (wfrec r H) r a) a"
+apply (simp add: wfrec_def)
+apply (rule adm_lemma [THEN wfrec_unique, THEN the1_equality], assumption)
+apply (rule wfrec_rel.wfrecI)
+apply (intro strip)
+apply (erule adm_lemma [THEN wfrec_unique, THEN theI'])
+done
+
+
+text{** This form avoids giant explosions in proofs.  NOTE USE OF ==*}
+lemma def_wfrec: "[| f==wfrec r H;  wf(r) |] ==> f(a) = H (cut f r a) a"
+apply auto
+apply (blast intro: wfrec)
+done
+
+
+subsection{*Variants for TFL: the Recdef Package*}
+
+lemma tfl_wf_induct: "ALL R. wf R -->  
+       (ALL P. (ALL x. (ALL y. (y,x):R --> P y) --> P x) --> (ALL x. P x))"
+apply clarify
+apply (rule_tac r = R and P = P and a = x in wf_induct, assumption, blast)
+done
+
+lemma tfl_cut_apply: "ALL f R. (x,a):R --> (cut f R a)(x) = f(x)"
+apply clarify
+apply (rule cut_apply, assumption)
+done
+
+lemma tfl_wfrec:
+     "ALL M R f. (f=wfrec R M) --> wf R --> (ALL x. f x = M (cut f R x) x)"
+apply clarify
+apply (erule wfrec)
+done
+
+subsection {*LEAST and wellorderings*}
+
+text{* See also @{text wf_linord_ex_has_least} and its consequences in
+ @{text Wellfounded_Relations.ML}*}
+
+lemma wellorder_Least_lemma [rule_format]:
+     "P (k::'a::wellorder) --> P (LEAST x. P(x)) & (LEAST x. P(x)) <= k"
+apply (rule_tac a = k in wf [THEN wf_induct])
+apply (rule impI)
+apply (rule classical)
+apply (rule_tac s = x in Least_equality [THEN ssubst], auto)
+apply (auto simp add: linorder_not_less [symmetric])
+done
+
+lemmas LeastI   = wellorder_Least_lemma [THEN conjunct1, standard]
+lemmas Least_le = wellorder_Least_lemma [THEN conjunct2, standard]
+
+lemma not_less_Least: "[| k < (LEAST x. P x) |] ==> ~P (k::'a::wellorder)"
+apply (simp (no_asm_use) add: linorder_not_le [symmetric])
+apply (erule contrapos_nn)
+apply (erule Least_le)
+done
+
+ML
+{*
+val wf_def = thm "wf_def";
+val wfUNIVI = thm "wfUNIVI";
+val wfI = thm "wfI";
+val wf_induct = thm "wf_induct";
+val wf_not_sym = thm "wf_not_sym";
+val wf_asym = thm "wf_asym";
+val wf_not_refl = thm "wf_not_refl";
+val wf_irrefl = thm "wf_irrefl";
+val wf_trancl = thm "wf_trancl";
+val wf_converse_trancl = thm "wf_converse_trancl";
+val wf_eq_minimal = thm "wf_eq_minimal";
+val wf_subset = thm "wf_subset";
+val wf_empty = thm "wf_empty";
+val wf_insert = thm "wf_insert";
+val wf_UN = thm "wf_UN";
+val wf_Union = thm "wf_Union";
+val wf_Un = thm "wf_Un";
+val wf_prod_fun_image = thm "wf_prod_fun_image";
+val acyclicI = thm "acyclicI";
+val wf_acyclic = thm "wf_acyclic";
+val acyclic_insert = thm "acyclic_insert";
+val acyclic_converse = thm "acyclic_converse";
+val acyclic_impl_antisym_rtrancl = thm "acyclic_impl_antisym_rtrancl";
+val acyclic_subset = thm "acyclic_subset";
+val cuts_eq = thm "cuts_eq";
+val cut_apply = thm "cut_apply";
+val wfrec_unique = thm "wfrec_unique";
+val wfrec = thm "wfrec";
+val def_wfrec = thm "def_wfrec";
+val tfl_wf_induct = thm "tfl_wf_induct";
+val tfl_cut_apply = thm "tfl_cut_apply";
+val tfl_wfrec = thm "tfl_wfrec";
+val LeastI = thm "LeastI";
+val Least_le = thm "Least_le";
+val not_less_Least = thm "not_less_Least";
+*}
 
 end
